Start working on pattern matching
Functions to determine if type is ADT and if so, to get params
Most of function to compile match valuation
Have ADT rep cast
Need proof of lengths (from type well-formedness), proof of uniformity
(from assumption)
Then whatever we need for arg_list

proofs/core/Denotational.v
@@ -330,6 +330,306 @@ Definition term_option_type (s: sig) (o: option term) (ty: vty) :=
   | None => True
   | Some t => term_has_type s t ty
   end.
+
+(*A not-as-typechecked version of [substi]*)
+(*Definition add_val (v: valuation gamma_valid i) (x: vsymbol) (vty: vty)
+Print valuation.
+
+Check substi.
+Print substi.
+Print Semantics.substi.
+
+Print valuation.*)
+
+Lemma existsb_exists': forall {A: Type} (f: A -> bool) (l: list A),
+  existsb f l = true -> {x | In x l /\ f x = true}.
+Proof.
+  intros. induction l; simpl in H. inversion H.
+  destruct (f a) eqn : Hf.
+  - exists a. split; auto. left; auto.
+  - specialize (IHl H). destruct IHl as [x [Hinx Hx]].
+    + apply (exist _ x). split; auto. right; auto.
+Qed.
+
+Check find.
+Search find.
+Locate find.
+
+Definition find_ts_in_mut (ts: typesym) (m: mut_adt) : option alg_datatype :=
+  find (fun a => typesym_eq_dec ts (adt_name a)) (typs m).
+
+Lemma find_ts_in_mut_some: forall ts m a,
+  find_ts_in_mut ts m = Some a ->
+  adt_in_mut a m /\ adt_name a = ts.
+Proof.
+  intros ts m a Hf. apply find_some in Hf.
+  destruct Hf as [Hin Heq].
+  split; auto.
+  simpl_sumbool.
+Qed.
+
+Set Bullet Behavior "Strict Subproofs".
+
+Lemma find_some_nodup: forall {A: Type} (f: A -> bool) (l: list A) (x: A),
+  (forall x y, In x l -> In y l -> f x -> f y -> x = y) ->  
+  (find f l = Some x <-> In x l /\ f x = true).
+Proof.
+  intros. induction l; intros; simpl; split; intros.
+  - inversion H0.
+  - destruct H0. destruct H0.
+  - destruct (f a) eqn : Hfa.
+    + inversion H0; subst. split; auto.
+    + apply IHl in H0. 
+      * destruct H0. split; auto.
+      * intros; apply H; auto; right; auto.
+  - destruct H0. destruct H0; subst. rewrite H1. reflexivity.
+    destruct (f a) eqn : Hfa.
+    + f_equal. apply H; auto. left; auto. right; auto.
+    + apply IHl; [|split; auto].
+      intros; apply H; auto; right; auto.
+Qed.
+
+Lemma NoDup_map_in: forall {A B: Type} {f: A -> B} {l: list A} {x1 x2: A},
+  NoDup (map f l) ->
+  In x1 l -> In x2 l ->
+  f x1 = f x2 ->
+  x1 = x2.
+Proof.
+  intros. induction l; simpl; intros; auto.
+  inversion H0.
+  simpl in H0; simpl in H1. simpl in H; inversion H; subst.
+  destruct H0; subst; destruct H1; subst.
+  - reflexivity.
+  - rewrite H2 in H5. exfalso. apply H5. rewrite in_map_iff. 
+    exists x2; split; auto.
+  - rewrite <- H2 in H5. exfalso. apply H5. rewrite in_map_iff.
+    exists x1; split; auto.
+  - apply IHl; auto.
+Qed.
+
+Lemma find_ts_in_mut_iff: forall ts m a,
+  NoDup (map adt_name (typs m)) ->
+  (find_ts_in_mut ts m = Some a) <-> (adt_in_mut a m /\ adt_name a = ts).
+Proof.
+  intros. eapply iff_trans. apply find_some_nodup.
+  - intros. repeat simpl_sumbool.
+    apply (NoDup_map_in H); auto.
+  - simpl. unfold adt_in_mut. apply and_iff_compat_l.
+    split; intros; simpl_sumbool.
+Qed.
+
+Definition find_ts_in_ctx (ts: typesym) : option (mut_adt * alg_datatype) :=
+  fold_right (fun m acc => 
+    match (find_ts_in_mut ts m) with
+    | Some a => Some (m, a)
+    | None => acc
+    end) None (mut_of_context gamma).
+
+(*TODO: move?*)
+Lemma no_adt_name_dups:
+  NoDup (map adt_name (concat (map typs (mut_of_context gamma)))).
+Proof.
+  assert (forall g, 
+    (map adt_name (concat (map typs (mut_of_context g)))) =
+  typesyms_of_context g). {
+    induction g; unfold typesyms_of_context in *; simpl; auto.
+    unfold datatypes_of_context in *.
+    destruct a; simpl; auto.
+    rewrite !map_app, IHg. f_equal.
+    rewrite map_map.
+    apply map_ext. intros a. destruct a; reflexivity.
+  }
+  rewrite H. apply gamma_valid.
+Qed.
+
+(*The real spec we want: (TODO: maybe move all this)*)
+Lemma find_ts_in_ctx_iff: forall ts m a,
+  (find_ts_in_ctx ts = Some (m, a) <-> mut_in_ctx m gamma /\
+    adt_in_mut a m /\ adt_name a = ts).
+Proof.
+  intros. unfold find_ts_in_ctx. rewrite mut_in_ctx_eq.
+  assert (forall m, In m (mut_of_context gamma) ->
+    NoDup (map adt_name (typs m))). {
+      intros m'. rewrite <- mut_in_ctx_eq.
+      eapply adts_names_nodups. apply gamma_valid.
+    }
+  assert (Hnodup:=no_adt_name_dups).
+  induction (mut_of_context gamma); simpl; intros; split; intros; auto.
+  - inversion H0.
+  - destruct H0 as [[] _].
+  - destruct (find_ts_in_mut ts a0) eqn : Hmut.
+    + inversion H0; subst. apply find_ts_in_mut_iff in Hmut. destruct Hmut.
+      repeat split; auto.
+      apply H. left; auto.
+    + apply IHl in H0. destruct H0 as [Hin [Ha Hn]]. repeat split; auto.
+      intros. apply H. right; auto.
+      simpl in Hnodup. rewrite map_app in Hnodup. apply NoDup_app in Hnodup.
+      apply Hnodup.
+  - destruct H0 as [[Ham | Hinm] [Ha Hn]]; subst.
+    + assert (find_ts_in_mut (adt_name a) m = Some a). {
+        apply find_ts_in_mut_iff. apply H. left; auto. split; auto.
+      }
+      rewrite H0. reflexivity.
+    + simpl in Hnodup. rewrite map_app in Hnodup.
+      rewrite NoDup_app_iff in Hnodup.
+      destruct (find_ts_in_mut (adt_name a) a0 ) eqn : Hf.
+      * apply find_ts_in_mut_iff in Hf. 2: apply H; simpl; auto.
+        destruct Hf.
+        destruct Hnodup as [Hn1 [Hn2 [Hi1 Hi2]]].
+        exfalso. apply (Hi1 (adt_name a1)). rewrite in_map_iff.
+        exists a1. split; auto. rewrite H1.
+        rewrite in_map_iff. exists a. split; auto.
+        rewrite in_concat. exists (typs m). split; auto.
+        rewrite in_map_iff. exists m; split; auto.
+      * apply IHl; auto.
+        intros. apply H. right; auto.
+        apply Hnodup.
+Qed.
+
+Definition vty_is_cons (v: vty) :=
+  match v with
+  | vty_cons _ _ => true
+  | _ => false
+  end.
+
+Lemma null_nil: forall {A: Type} (l: list A),
+  null l <-> l = nil.
+Proof.
+  intros; destruct l; split; intros; auto; inversion H.
+Qed.
+
+Lemma is_sort_cons: forall (ts: typesym) (l: list vty),
+  is_sort (vty_cons ts l) ->
+  forall x, In x l -> is_sort x.
+Proof.
+  intros. unfold is_sort in *. simpl in H.
+  rewrite null_nil in *.
+  eapply big_union_nil in H. apply H. assumption.
+Qed.
+
+Definition is_sort_cons_sorts (ts: typesym) (l: list vty) 
+  (Hall: forall x, In x l -> is_sort x):
+  {s: list sort | sorts_to_tys s = l}.
+Proof.
+  induction l.
+  - apply (exist _ nil). reflexivity.
+  - simpl in Hall.
+    assert (is_sort a). apply Hall. left; auto.
+    assert (forall x : vty, In x l -> is_sort x). {
+      intros. apply Hall; right; auto.
+    }
+    specialize (IHl H0). destruct IHl as [tl Htl].
+    apply (exist _ ((exist _ a H) :: tl)).
+    simpl. rewrite Htl. reflexivity.
+Qed.
+(*
+Definition sort_cons (t: typesym) (l: list vty) (Hsrt: is_sort (vty_cons t l)) :
+  { s: list sort | 
+    vty_cons t  = vty_cons (fst t) (sorts_to_tys (snd t))}
+| _ => unit
+end.
+Proof.
+  destruct s. simpl. destruct x; try solve[apply tt].
+  pose proof (is_sort_cons_sorts t l (is_sort_cons t l i0)) as ls.
+  destruct ls as [s Hs].
+  apply (exist _ (t, s)). simpl. rewrite Hs. reflexivity.
+Qed.*)
+
+Definition is_sort_adt (s: sort) : 
+  option (mut_adt * alg_datatype * typesym * list sort).
+Proof.
+  destruct s.
+  destruct x.
+  - exact None.
+  - exact None.
+  - exact None.
+  - destruct (find_ts_in_ctx t);[|exact None].
+    exact (Some (fst p, snd p, t, 
+      proj1_sig (is_sort_cons_sorts t l (is_sort_cons t l i0)))).
+Defined.
+
+(*TODO: do we need other direction?*)
+Lemma is_sort_adt_spec: forall s m a ts srts,
+  is_sort_adt s = Some (m, a, ts, srts) ->
+  s = typesym_to_sort (adt_name a) srts /\
+  adt_in_mut a m /\ mut_in_ctx m gamma /\ ts = adt_name a.
+Proof.
+  intros. unfold is_sort_adt in H.
+  destruct s. destruct x; try solve[inversion H].
+  destruct (find_ts_in_ctx t) eqn : Hf.
+  - inversion H; subst. destruct p as [m a]. simpl.
+    apply find_ts_in_ctx_iff in Hf. destruct Hf as [Hmg [Ham Hat]]; 
+    repeat split; auto; subst.
+    apply sort_inj. simpl. f_equal. clear H. 
+    generalize dependent (is_sort_cons (adt_name a) l i0).
+    intros H.
+    destruct (is_sort_cons_sorts (adt_name a) l H). simpl.
+    rewrite <- e; reflexivity.
+  - inversion H.
+Qed.
+
+Check find_constr_rep.
+Print pre_interp.
+Check adts.
+
+(*We handle pattern matches slightly differently than in the paper.
+  We build up a complete valuation that binds all of the pattern
+  variables to the domain values, then interpret the resulting term
+  or formula using this valuation. We provide a function that gives
+  the valuation and the term/formula to abstract out the common
+  functionality.*)
+Fixpoint match_val_single (v: valuation gamma_valid i) (ty: vty)
+  (d: domain (val v ty))
+  (p: pattern) : option (valuation gamma_valid i) :=
+  match p with
+  | Pvar x _ => Some (substi v x ty d)
+  | Pwild => Some v
+  | Por p1 p2 => match (match_val_single v ty d p1) with
+                  | Some v1 => Some v1
+                  | None => match_val_single v ty d p2
+                  end
+  | Pbind p1 x _ => match_val_single (substi v x ty d) ty d p1 
+    (*TODO: is this right - do we evaluation pattern with additional binding?*)
+  | Pconstr f vs ps =>
+    match (is_sort_adt (val v ty)) as o return
+      (is_sort_adt (val v ty)) = o -> option (valuation gamma_valid i)
+    with
+    | Some (m, a, ts, srts) => fun Hisadt =>
+      (*So now (with result about, we know that sort is ADT)*)
+      (*Now we need to cast this to adt_rep*)
+      (*First, get info about a, m, srts from [is_sort_adt_spec]*)
+      match (is_sort_adt_spec _ _ _ _ _ Hisadt) with
+      | conj Hseq (conj a_in (conj m_in Htseq)) =>
+        (*We cast to get an ADT, now that we know that this actually is
+          an ADT*)
+        let adt : adt_rep m srts (dom_aux gamma_valid i) a a_in :=
+          scast (adts gamma_valid i m srts a a_in) (dom_cast _ Hseq d) in
+          None
+        (*TODO: need to know that length of srts is correct - need to know
+          that type itself is well-typed (then use separate lemma to show
+          this, need to know that args are same for all which I believe is
+          current assumption)*)
+        (*let f := find_constr_rep gamma_valid m m_in srts (*TODO*) _ 
+          _ a a_in (adts gamma_valid i m srts a a_in)*)
+          (*TODO: need uniformity*)
+          (*TODO: need to cast this to [adt_rep m srts domain_aux a a_in]*)
+      (*let f := find_constr_rep gamma_valid m *)
+      end 
+
+
+
+      
+    | None => fun _ => None
+    end eq_refl
+    (*Idea: see if sort is ADT - need function to do this + get parts*)
+    (*if not, give None*)
+    (*if so, get constr_rep and see if equals f, if not None*)
+    (*if equals f, then take arg list, eval list of patterns on this
+      will need to know that this is (val v ty) for each ty - hopefully
+      not too hard to show*)
+  end.
+
+
 (*First, we handle matches - we will take in isf and projf as predicates
   and give them later - TODO: hopefully it works*)
 (*This makes dependent types much nicer*)
